# Parsers

Studied top down parsers. Here are 2 which I studied -

## Recursive descent parser

Used to parse a expression from left to right according to a certain **context free grammar**, using a recursive approach of backtracking when a terminal is matched/reached.

Here's an example for a recursive descent parser for a C-type **for-loop** -

        Designed grammar (CFG) for this construct 
 
        G = {{S, E, B, I, C}, {for, (, ), ;, =, a, k, ε, {, }, <, >, +, -}, {P}, S}
 
        Where P (set of productions) is -
 
        S -> for(E;E;I)B
        E -> a=k|aCk|ε
        B -> {I;}
        I -> a++|a--|++a|--a
        C -> >|<|==

Code for recursive descent parser for this grammar in C -

```C

#include <stdio.h>
#include <string.h>
 
void S();
void E();
void B();
void I();
void C();
char getInput[50];
int i, error;
 
int main()
{
	FILE *fp;
 
	fp = fopen("inputfor.txt", "r");
	fgets(getInput, sizeof(getInput), fp);
	strtok(getInput, "\n");
 
	printf("%s\n", getInput);
	S();
	if (i == strlen(getInput) && error == 0)
	{
		printf("Valid Expression : No Syntax Error \n");
	}
	else
	{
		printf("Invalid Expression : Syntax Error; At position %d\n", i);
	}
}
 
void S()
{
	if(getInput[i] == 'f' && (getInput[i+1] == 'o' && getInput[i+2] == 'r'))
	{
		i += 3;
		if(getInput[i] == '(') 
		{
			i++;
			E();
			if (getInput[i] == ';') 
			{
				i++;
				E();
				if (getInput[i] == ';') 
				{
					i++;
					I();
					if (getInput[i] == ')') 
					{
						i++;
						B();
					}
					else 
					{
						error = 1;
					}
				}
				else 
				{
					error = 1;
				}
			}
			else 
			{
				error = 1;
			}
		}
		else 
		{
			error = 1;
		}
	}
	else 
	{
		error = 1;
	}
}
 
void E() 
{
	if (getInput[i] == 'a' && (getInput[i+1] == '=' && getInput[i+2] == 'k')) 
	{
		i += 3;
	}
	else if (getInput[i] == 'a' && getInput[i + 1] != '=') 
	{
		i++;
		C();
		if(getInput[i] == 'k') 
		{
			i++;
		}
	}
}
 
void I() 
{
	bool cond1 = getInput[i] == 'a' && (getInput[i + 1] == '+' && getInput[i + 2] == '+');
	bool cond2 = getInput[i] == 'a' && (getInput[i + 1] == '-' && getInput[i + 2] == '-');
	bool cond3 = getInput[i] == '+' && (getInput[i + 1] == '+' && getInput[i + 2] == 'a');
	bool cond4 = getInput[i] == '-' && (getInput[i + 1] == '-' && getInput[i + 2] == 'a');
 
	if (cond1 || (cond2 || (cond3 || cond4))) 
	{
		i += 3;
	}
}
 
void C() 
{
	if (getInput[i] == '<' || getInput[i] == '>') 
	{
		i++;
	}
	else if (getInput[i] == '=' && getInput[i + 1] == '=') 
	{
		i += 3;
	}
	else 
	{
		error = 1;
	}
}
 
void B() 
{
	if (getInput[i] == '{') 
	{
		i++;
		I();
		if (getInput[i] == ';') 
		{
			i++;
		}
		if(getInput[i] == '}') 
		{
			i++;
		}
		else 
		{
			error = 1;
		}
	}
}


```

## Predictive descent parser

Predictive descent parser or LL(k) parser, where k is the number tokens considered for lookahead. This is basically a form of recursive descent parser that doesn't need backtracking for evaluating input to a certain context free grammar. 

Here, the `LL` implies "**L**eft to right" for L and "**L**eftmost derivation" for L. As is understandable, there is a LR parser too, and here the `LR` means "**L**eft to right" for L and "**R**ightmost derivation in reverse" for R.

Key difference is that `LL` parsers are top down parsers, while `LR` parsers are bottom up parsers.

Here is an example for a LL(1) parser for an expression with '+' and '*' operators only.

```

Designed grammar (CFG) for this construct 
G = {{E, T, E',T', F}, {(, ), ε, +, *, id}, {P}, E}

where P is set below set of productions 

E -> TE'
E'-> +TE'|ε
T -> FT'
T'-> *FT'|ε
F -> (E)|id

```

Code for LL(1) parser for this grammar in C -

```C

#include <stdio.h>
#include <stdlib.h>
#include <string.h>
#include <ctype.h>

void E();
void T();
void F();
void match(char t);
void error();
char lookahead;
int i = 0, err = 0;
char getInput[50];

int main()
{
	FILE *fp;

	fp = fopen("input-diff.txt", "r");
	fgets(getInput, sizeof(getInput), fp);
	strtok(getInput, "\n");

	printf("%s\n", getInput);

	lookahead = getInput[i];
	E();

	printf("\nValid Expression : No Syntax Error \n");
}

void E()
{
	T();
	while (1)
	{
		if (lookahead == '+')
		{
			match(lookahead);
			T();
		}
		else { break; }
	}
}

void T()
{
	F();
	while(1) 
	{
		if (lookahead == '*')
		{
			match(lookahead);
			F();
		}
		else { break; }
	}
}

void F()
{
	if (isdigit(lookahead))
	{
		while (isdigit(lookahead))
		{
			match(lookahead);
		}
	}
	else if (lookahead == '(')
	{
		match(lookahead);
		E();
		if (lookahead == ')')
		{
			match(lookahead);
		}
		else
		{
			error();
		}
	}
	else
	{
		error();
	}
}

void error()
{
	printf("\nSyntax error at %d\n", i);
	exit(1);
}

void match(char t)
{
	if (lookahead == t)
	{
		printf("%c", t);
		i++;
		lookahead = getInput[i];
	}
	else error();
}

```

You will see in the code that we have a while loop, which actually replaces a tail recursion that might have been there in case we were writing a recursive parser. We can get the idea for the recursive call by studying the grammar. You will see that both T' and F' have a self pointing production. This would have led to a tail recursion but we avoided that this way.

